c0

syntax.v
@@ -3,279 +3,38 @@ Require Import List.
 Require Import Nat.
 Import ListNotations.
 
-
 Definition VarT := string.
-Definition ValT := nat.
-(* Variable (Addr:Type) (AddrEq: forall (x y:Addr), {x=y} + {x<>y}). *)
 Definition Addr := nat.
-Definition AddrEq := PeanoNat.Nat.eq_dec.
+Variant Val :=
+    | AddrVal (addr: Addr)
+    | IntVal (v: nat).
 
-Variant AOp :=
-    | Add
-    | Sub
-    | Mul
-    .
+Variant Op := 
+    Add | Mul.
 
-Variant COp :=
-    | Eq
-    | Lt
-    .
+    (* Lt Eq *)
 
-Variant Op :=
-    | ArithOp (op:AOp)
-    | CompOp (op:COp)
-    .
-
-Inductive Val :=
-    | NumVal (n:ValT)
-    | AddrVal (a:Addr)
-    .
-
-Inductive LExpr :=
-    | Var (x:VarT)
-    (* C0p *)
-    | Indir (e:Expr)
-with Expr :=
+Inductive Expr :=
     | Const (c:Val)
-    | Left (e:LExpr)
-    | Binary (op:Op) (e1:Expr) (e2:Expr)
-    (* C0p *)
-    | Adress (l:LExpr)
+    | Binary (o:Op) (e1 e2:Expr)
+    | LVal (l:LExpr)
+with LExpr :=
+    | Var (v:VarT)
     .
 
-Variant ITy :=
-    | Char
-    | Int.
-
-Inductive PTy :=
-    | Ptr (t:Ty)
-with STy :=
-    | PtrScal (p:PTy)
-    | IntScal (i:ITy)
-with Ty :=
-    | Scal (s:STy)
-    | Void
-    .
+Implicit Type (e : Expr) (c : Val) (x y : VarT).
 
 Inductive Stmt :=
-    | Assign (l:LExpr) (e:Expr)
-    | If (e:Expr) (s1:Stmt) (s2:Stmt)
-    | While (e:Expr) (s:Stmt)
-    (* | Block (s:list Stmt) *)
+    (* | Assume e *)
+    (* | Assert e *)
+    | While e (s:Stmt)
+    | If e (s_then s_else : Stmt)
+    | Block (h:list Stmt)
+    | Assign (x:LExpr) e
     | Abort
-    (* C0b *)
-    | Block (decl:list (STy*VarT)) (s:list Stmt)
     .
 
-Variant UndefVal :=
-    | Undef
-    | Defined (v:Val)
-    .
-
-Notation VarEnv := (VarT -> option Addr).
-Notation MemEnv := (Addr -> UndefVal).
-
-Record State :=
-    {
-        var_assign: VarEnv;
-        memory_assign: MemEnv
-    }.
-
-Variant Conf :=
-    | Aborted
-    | Terminated (s:State)
-    | Running (smt:Stmt) (s:State)
-    .
-
-Notation "⟨ s | o ⟩" := (Running s o).
-Coercion Terminated : State >-> Conf.
-Notation Env := 
-    (fun σ =>
-    let '(ρ,μ) := σ in
-    Build_State ρ μ).
-Coercion Defined : Val >-> UndefVal.
-
-Load option_monad.
-
-Definition LExprEval (l:LExpr) (s:State) : option Addr :=
-    let (ρ,μ) := s in
-    match l with 
-    | Var x =>
-        ρ x
-    | Indir e => None
-    (* TODO C0p *)
-    end
-    .
-Fixpoint ExprEval (e:Expr) (s:State) : option Val :=
-    match e with 
-    | Const c => ret c
-    | Left l => 
-        let (ρ,μ) := s in
-        t <- LExprEval l s;;
-        match (μ t) with 
-        | Undef => None
-        | Defined v =>
-            ret v
-        end
-    | Binary op e1 e2 =>
-        v1 <- ExprEval e1 s;;
-        v2 <- ExprEval e2 s;;
-        match v1,v2,op with
-        | NumVal n1, NumVal n2, ArithOp Add => ret (NumVal (n1 + n2))
-        | NumVal n1, NumVal n2, ArithOp Sub => ret (NumVal (n1 - n2))
-        | NumVal n1, NumVal n2, ArithOp Mul => ret (NumVal (n1 * n2))
-        | NumVal n1, NumVal n2, CompOp Eq => ret (if n1 =? n2 then NumVal 1 else NumVal 0)
-        | NumVal n1, NumVal n2, CompOp Lt => ret (if n1 <? n2 then NumVal 1 else NumVal 0)
-        | _, _, _ => None
-        end
-    | Adress l =>
-        None (* TODO C0p *)
-    end
-    .
-
-
-Definition update {A B} {Aeq:forall a b, {a=b} + {a<>b}} (f:A -> B) (x:A) (y:B) (x2:A) : B :=
-        if Aeq x x2 then y else f x2.
-
-Definition Skip := Block [] [].
-
-    (* page 140 *)
-Reserved Notation "c1 ~> c2" (at level 40).
-(* TODO: C0b *)
-Inductive step : Conf -> Conf -> Prop :=
-    | EmptyStep σ: ⟨ Skip | σ ⟩ ~> σ
-    | AssignStep ρ μ l e v a: 
-        ExprEval e (Env (ρ,μ)) = Some v ->
-        LExprEval l (Env (ρ,μ)) = Some a ->
-        ⟨ Assign l e | Env (ρ,μ) ⟩ ~> 
-        Env (ρ, @update _ _ AddrEq μ a (Defined v))
-    | IfTrueStep σ e s1 s2 n: 
-        ExprEval e σ = Some (NumVal n) ->
-        n <> 0 ->
-        ⟨ If e s1 s2 | σ ⟩ ~> ⟨ s1 | σ ⟩
-    | IfFalseStep σ e s1 s2: 
-        ExprEval e σ = Some (NumVal 0) ->
-        ⟨ If e s1 s2 | σ ⟩ ~> ⟨ s2 | σ ⟩
-    | WhileStep σ e s: 
-        ⟨ While e s | σ ⟩ ~> 
-        ⟨ If e (Block [] [s; While e s]) Skip | σ ⟩
-    | AbortStep σ : ⟨ Abort | σ ⟩ ~> Aborted
-    | ExecStep σ (σ':State) s1 sr:
-        ⟨ s1 | σ ⟩ ~> σ' ->
-        ⟨ Block [] (s1::sr) | σ ⟩ ~> 
-        ⟨ Block [] sr | σ' ⟩
-    | CrashStep σ s1 sr:
-        ⟨ s1 | σ ⟩ ~> Aborted ->
-        ⟨ Block [] (s1::sr) | σ ⟩ ~> Aborted
-    | SubstStep σ (σ':State) s1 s1' sr:
-        ⟨ s1 | σ ⟩ ~> ⟨ s1' | σ' ⟩ ->
-        ⟨ Block [] (s1::sr) | σ ⟩ ~> 
-        ⟨ Block [] (s1'::sr) | σ' ⟩
-    where "c1 ~> c2" := (step c1 c2).
-
-Definition final c := ~exists c2, c ~> c2.
-
-Reserved Notation "c1 ⇓ c2" (at level 40).
-Inductive big_step : Conf -> Conf -> Prop :=
-    | BigStepEnd c:
-        final c ->
-        c ⇓ c
-    | BigStepTrans c1 c2 c3:
-        c1 ~> c2 ->
-        c2 ⇓ c3 ->
-        c1 ⇓ c3
-    where "c1 ⇓ c2" := (big_step c1 c2).
+Implicit Type (ss : list Stmt) (s:Stmt).
 
 
 
-    (* 149 => static sema *)
-
-    (* Hoare 156 *)
-
-Require Import String.
-Local Open Scope string_scope.
-
-Require Import Lia.
-
-Goal forall a b, a<=b <-> a < S b.
-Proof.
-intros;split;intros;lia.
-Qed.
-
-Definition example5_5 :=
-    Block [
-        (* (Int, "x"),
-        (Int, "y"),
-        (Int, "z") *)
-    ] [
-        Assign (Var "q") (Const (NumVal 0));
-        Assign (Var "r") (Left (Var "x"));
-        While (Binary (CompOp Lt) (Left (Var "y")) (Binary (ArithOp Add) (Const (NumVal 1)) (Left (Var "r")))) (
-            Block [
-            ] [
-                Assign (Var "r") (Binary (ArithOp Sub) (Left (Var "r")) (Const (NumVal 1)));
-                Assign (Var "q") (Binary (ArithOp Add) (Left (Var "q")) (Const (NumVal 1)))
-            ]
-        )
-    ]
-    .
-
-Definition empty_env {A B} (x:A) : option B := None.
-
-Fixpoint to_single_env {A B AEq} (xs:list (A*B)) :=
-    match xs with 
-    | [] => empty_env
-    | (a,b)::xr => @update _ _ AEq (@to_single_env A B AEq xr) a (Some b)
-    end.
-
-
-Fixpoint to_env_aux (xs:list (VarT*UndefVal)) :=
-    match xs with 
-    | [] => (empty_env, fun _ => Undef, 0)
-    | (a,b)::xr => 
-        let '(addr_map, val_map, n) := to_env_aux xr in
-        let addr := 1000+n in
-            (@update _ _ string_dec addr_map a (Some addr), @update _ _ AddrEq val_map addr b, S n)
-    end.
-
-Definition to_env xs :=
-    let '(ρ,μ,n) := to_env_aux xs in
-    Env (ρ,μ).
-
-(* Notation "{ }" := empty_env (format "{ }").
-Notation "{ x ↦ v }" := (update empty_env x v).
-Notation "[ x ↦ v ; y ↦ w ; .. ; z ↦ r ]" := (update (update (.. (update empty_env z r) ..) y w ) x v). *)
-
-
-
-
-(* Goal ⟨ example5_5 | to_env [("q", Undef); ("r",Undef); ("x", Defined(NumVal 5)); ("y", Defined(NumVal 2))] ⟩ ⇓ 
-    to_env [("q", Defined( NumVal 2)); ("r",Defined(NumVal 1)); ("x", Defined(NumVal 5)); ("y", Defined(NumVal 2))].
-Proof.
-    cbn.
-    do 12 (eapply BigStepTrans;[shelve|]).
-    Unshelve.
-    1-13: shelve.
-    - apply ExecStep.
-      apply AssignStep;now cbn.
-    - apply ExecStep.
-      apply AssignStep;cbn.
-      all: reflexivity.
-      (* unfold ExprEval.
-      cbn [LExprEval].
-      remember (update _ _ _ _).
-      cbn in Heqy.
-      1: cbn.
-      2: cbn. *)
-    - apply SubstStep.
-      apply WhileStep.
-    - apply SubstStep.
-      eapply IfTrueStep;[vm_compute|].
-      all: auto.
-    - apply ExecStep.
-      constructor.
-      apply AssignStep.
-      apply ExecStep.
-      apply SubstStep.
-      (* cbn [ExprEval].
-      cbn [ExprEval LExprEval bind ret]. *) *)
