semantics.v
@@ -1,0 +1,208 @@
+Load syntax.
+
+Variant UndefVal :=
+    | Undef
+    | Defined (v:Val)
+    .
+
+Notation VarEnv := (VarT -> option Addr).
+Notation MemEnv := (Addr -> option UndefVal).
+
+(* Record State :=
+    {
+        var_assign: VarEnv;
+        memory_assign: MemEnv
+    }. *)
+Definition State := (VarEnv * MemEnv)%type.
+
+Implicit Type (ρ:VarEnv) (μ:MemEnv) (σ:State).
+
+Load option_monad.
+
+Definition lookupVar σ x :=
+    let (ρ, μ) := σ in 
+    a <- ρ x;;
+    μ a.
+
+Definition LExprEval (l:LExpr) (σ:State) : option Addr :=
+    let (ρ,μ) := σ in
+    match l with
+    | Var x => ρ x
+    end.
+Definition evalOp (op:Op) (v1 v2:Val) : option Val :=
+    None.
+    (* match op,v1,v2 with
+    | Add, Undef, Undef => Undef *)
+Fixpoint ExprEval (e:Expr) (s:State) : option Val :=
+    match e with 
+    | Const c => ret c
+    | LVal l => 
+        let (ρ,μ) := s in
+        a <- LExprEval l s;;
+        uv <- μ a;;
+        match uv with 
+        | Undef => None
+        | Defined v =>
+            ret v
+        end
+    | Binary op e1 e2 =>
+        v1 <- ExprEval e1 s;;
+        v2 <- ExprEval e2 s;;
+        evalOp op v1 v2
+    end
+    .
+
+
+Variant Conf :=
+    | Aborted
+    | Terminated (s:State)
+    | Running (smt:Stmt) (s:State)
+    .
+
+
+Class EqDec (A:Type) :=
+    {eqdec:(forall (x y:A), {x = y} + {x<>y})}.
+
+Definition update {A B} {Aeq:EqDec A} (f:A -> B) (x:A) (y:B) (x2:A) : B :=
+        if @eqdec A Aeq x x2 then y else f x2.
+
+Instance AddrEq : EqDec Addr.
+    constructor.
+    now decide equality.
+Defined.
+
+
+Notation RExprEval := ExprEval.
+
+Notation "⟨ s | st ⟩" := (Running s st).
+Notation "« st »" := (Terminated st).
+Notation "R⟦ e ⟧ σ" := (ExprEval e σ) (at level 40).
+Notation "L⟦ l ⟧ σ" := (LExprEval l σ) (at level 40).
+Notation "↯" := (Aborted).
+Coercion Terminated : State >-> Conf.
+Definition bool_to_nat (b:bool) := 
+    if b then 1 else 0.
+Coercion bool_to_nat : bool >-> nat.
+Coercion IntVal : nat >-> Val.
+Coercion Defined : Val >-> UndefVal.
+(* Coercion Some : UndefVal >-> (option UndefVal). *)
+
+Reserved Notation "c1 ~> c2" (at level 50).
+Inductive step : Conf -> Conf -> Prop :=
+    | AssignStep l e ρ μ a v: 
+        let σ := (ρ, μ) in
+        R⟦e⟧σ = Some v ->
+        L⟦l⟧σ = Some a ->
+        ⟨ (Assign l e) | σ ⟩ ~> «(ρ, update μ a (Some (Defined v)))»
+    | IfTrueStep e s1 s2 σ (n:nat) :
+        R⟦e⟧σ = Some (n:Val) ->
+        n <> 0 ->
+        ⟨ (If e s1 s2) | σ ⟩ ~> ⟨ s1 | σ ⟩
+    | IfFalseStep e s1 s2 σ :
+        R⟦e⟧σ = Some (0:Val) ->
+        ⟨ (If e s1 s2) | σ ⟩ ~> ⟨ s1 | σ ⟩
+    | WhileStep e s σ (n:nat) :
+        ⟨ (While e s) | σ ⟩ ~> ⟨ If e (Block [s; While e s]) (Block []) | σ ⟩
+    | EmptyStep σ :
+        ⟨ Block [] | σ ⟩ ~> « σ »
+    | ExecStep s1 sr σ σ' :
+        ⟨ s1 | σ ⟩ ~> « σ' » ->
+        ⟨ Block (s1::sr) | σ ⟩ ~> ⟨ Block sr | σ' ⟩
+    | SubstStep s1 s1' sr σ σ' :
+        ⟨ s1 | σ ⟩ ~> ⟨ s1' | σ ⟩ ->
+        ⟨ Block (s1::sr) | σ ⟩ ~> ⟨ Block (s1'::sr) | σ' ⟩
+    | AbortStep σ :
+        ⟨ Abort | σ ⟩ ~> ↯
+    | CrashStep s1 sr σ :
+        ⟨ s1 | σ ⟩ ~> ↯ ->
+        ⟨ Block (s1::sr) | σ ⟩ ~> ↯
+    where "c1 ~> c2" := (step c1 c2).
+
+Inductive trace : list Conf -> Prop :=
+    | TraceEmpty : trace []
+    | TraceSingle (c:Conf) : trace [c]
+    | TraceCons : forall (c c':Conf) cs,
+        step c c' ->
+        trace (c'::cs) ->
+        trace (c::c'::cs).
+
+Definition terminal (c:Conf) :=
+    ~(exists (c':Conf), c ~> c').
+
+Reserved Notation "conf1 ⇓ conf2" (at level 50).
+Inductive bigStep : Conf -> Conf -> Prop :=
+    | BigStepEnd (c1:Conf) :
+        terminal c1 ->
+        c1 ⇓ c1
+    | BigStepTrans (c1 c2 c3:Conf):
+        c1 ~> c2 ->
+        c2 ⇓ c3 ->
+        c1 ⇓ c3
+    where "conf1 ⇓ conf2" := (bigStep conf1 conf2).
+
+Definition properTerm s σ σ' :=
+    ⟨ s | σ ⟩ ⇓ σ'.
+Definition abortion s σ :=
+    ⟨ s | σ ⟩ ⇓ ↯.
+Definition stuck s σ s' σ' :=
+    ⟨ s | σ ⟩ ⇓ ⟨ s' | σ' ⟩.
+
+
+Lemma terminalTerminated :
+    forall (σ:State),
+    terminal (Terminated σ).
+Proof.
+    intros.
+    intros [c' H].
+    inversion H.
+Qed.
+
+Definition isWhile s :=
+    match s with
+    | While e s => True
+    | _ => False
+    end.
+
+Goal forall l e σ,
+let s := Assign l e in
+    (exists σ', properTerm s σ σ') \/
+    (exists s' σ', stuck s σ s' σ').
+Proof.
+  intros x e σ;cbn.
+  destruct (R⟦ e ⟧ σ) eqn:He, (L⟦ x ⟧ σ) eqn:Hx;
+  destruct σ as [ρ μ]. 
+  2-4: 
+    right; exists (Assign x e); exists (ρ,μ);
+    apply BigStepEnd; intros [c' H];
+    inversion H;subst; subst σ0; congruence.
+  left.
+  eexists. 
+  eapply BigStepTrans.
+  * apply AssignStep;now eassumption.
+  * apply BigStepEnd. apply terminalTerminated.
+Qed.
+
+Goal forall σ,
+    abortion (Abort) σ.
+Proof.
+    intros.
+    eapply BigStepTrans;[constructor|apply BigStepEnd].
+    intros [c H];inversion H.
+Qed.
+
+(* bigstep only for statement and conf *)
+(* Reserved Notation "s , σ ⇓ conf" (at level 50).
+Inductive bigStep (s:Stmt) σ : Conf -> Prop :=
+    (* not necessary *)
+    | BigStepEnd :
+        (~exists (c2:Conf), step ⟨ s | σ ⟩ c2) ->
+        s, σ ⇓ ⟨ s | σ ⟩
+    | BigStepFinal (c1:Conf): 
+        step ⟨ s | σ ⟩ c1 ->
+        (~exists (c2:Conf), step c1 c2) ->
+        s, σ ⇓ c1
+    | BigStepTrans (c1):
+        step ⟨ s | σ ⟩ c1 ->
+
+    where "s , σ ⇓ conf" := (bigStep s σ conf).
+ *)
